Intermediate/Machine.v
@@ -231,16 +231,16 @@ Definition linkable_programs (p1 p2: program) : Prop :=
   PMapExtra.Disjoint (prog_interface p1) (prog_interface p2) /\
   (*  the sets of components having buffers are disjoint *)
   PMapExtra.Disjoint (prog_buffers p1) (prog_buffers p2) /\
-  (* ^ APT added 
-     Need something like this in order to prove linking_well_formedness, 
+  (* ^ APT added
+     Need something like this in order to prove linking_well_formedness,
      for example the buffers_existence clause.  Interface disjointness is not enough.
      For suppose C is in interface of p1 (hence not in interface of p2) but has buffers defined in p2
      (about which we know nothing).  Since p2 wins over p1 when combining buffers, we have to show
      that these p2 buffers are the required ones, which we don't know. *)
   (* the sets of components having procedures are disjoint *)
   PMapExtra.Disjoint (prog_procedures p1) (prog_procedures p2) /\
-  (* ^ APT added 
-     For similar reasons, needed to prove exported_procedures_existence. *)  
+  (* ^ APT added
+     For similar reasons, needed to prove exported_procedures_existence. *)
   (* the union of their interfaces is sound *)
   sound_interface (PMapExtra.update (prog_interface p1) (prog_interface p2)).
 
@@ -249,6 +249,15 @@ Definition program_link (p1 p2: program) mainC mainP : program :=
      prog_procedures := PMapExtra.update (prog_procedures p1) (prog_procedures p2);
      prog_buffers := PMapExtra.update (prog_buffers p1) (prog_buffers p2);
      prog_main := (mainC, mainP) |}.
+
+Definition partialize_program (p: program) (ctx: Program.interface) : program :=
+  {| prog_interface :=
+       PMapExtra.filter (fun k _ => negb (PMap.mem k ctx)) (prog_interface p);
+     prog_procedures :=
+       PMapExtra.filter (fun k _ => negb (PMap.mem k ctx)) (prog_procedures p);
+     prog_buffers :=
+       PMapExtra.filter (fun k _ => negb (PMap.mem k ctx)) (prog_buffers p);
+     prog_main := prog_main p |}.
 
 (*
 Ltac inv H := (inversion H; subst; clear H).
@@ -259,44 +268,44 @@ Theorem linking_well_formedness:
     linkable_programs p1 p2 ->
     well_formed_program (program_link p1 p2 mainC mainP).
 Proof.
-  intros. destruct H as (WF1 & WF2 & IDISJ & BDISJ & PDISJ & SND). 
-  constructor. 
-  + auto. 
-  + simpl. 
-    intros. 
+  intros. destruct H as (WF1 & WF2 & IDISJ & BDISJ & PDISJ & SND).
+  constructor.
+  + auto.
+  + simpl.
+    intros.
     rewrite PMapExtra.update_in_iff in H.
-    inv H. 
+    inv H.
     - destruct WF1. pose proof (wfprog_buffers_existence0 C H0).
-      clear - H BDISJ. unfold has_required_local_buffers in *. simpl. 
+      clear - H BDISJ. unfold has_required_local_buffers in *. simpl.
       destruct H as (b1 & b2 & bufs & FND & B1 & B2).
-      exists b1, b2, bufs. 
+      exists b1, b2, bufs.
       intuition.
-      rewrite <- PMapFacts.find_mapsto_iff in FND|-*.  
-      rewrite PMapExtra.update_mapsto_iff.  
+      rewrite <- PMapFacts.find_mapsto_iff in FND|-*.
+      rewrite PMapExtra.update_mapsto_iff.
       right.
       intuition.
-      eapply BDISJ. 
+      eapply BDISJ.
       split; [| apply H].
-      rewrite PMapFacts.find_mapsto_iff in FND.  
+      rewrite PMapFacts.find_mapsto_iff in FND.
       rewrite PMapFacts.in_find_iff.
       rewrite FND. discriminate.
     - destruct WF2. pose proof (wfprog_buffers_existence0 C H0).
-      clear - H BDISJ. unfold has_required_local_buffers in *. simpl. 
+      clear - H BDISJ. unfold has_required_local_buffers in *. simpl.
       destruct H as (b1 & b2 & bufs & FND & B1 & B2).
-      exists b1, b2, bufs. 
+      exists b1, b2, bufs.
       intuition.
-      rewrite <- PMapFacts.find_mapsto_iff in FND|-*.  
-      rewrite PMapExtra.update_mapsto_iff.  
+      rewrite <- PMapFacts.find_mapsto_iff in FND|-*.
+      rewrite PMapExtra.update_mapsto_iff.
       left.
       intuition.
-  + simpl. intros. 
-    rewrite PMapExtra.update_mapsto_iff in H. 
+  + simpl. intros.
+    rewrite PMapExtra.update_mapsto_iff in H.
     inv H.
-    - destruct WF2. 
+    - destruct WF2.
       edestruct wfprog_exported_procedures_existence0 as [cprocs [pcode [Q1 Q2]]]; eauto.
       exists cprocs, pcode. intuition.
       rewrite  PMapExtra.update_mapsto_iff. intuition.
-    - inv H1. destruct WF1. 
+    - inv H1. destruct WF1.
       edestruct wfprog_exported_procedures_existence0 as [cprocs [pcode [Q1 Q2]]]; eauto.
       exists cprocs, pcode. intuition.
       rewrite PMapExtra.update_mapsto_iff. right. intuition.
@@ -304,16 +313,16 @@ Proof.
       rewrite PMapFacts.find_mapsto_iff in Q1.
       rewrite PMapFacts.in_find_iff. rewrite Q1. discriminate.
   + simpl. intros.
-    rewrite PMapExtra.update_mapsto_iff in H. 
-    inv H. 
+    rewrite PMapExtra.update_mapsto_iff in H.
+    inv H.
     - destruct WF2.
       pose proof (wfprog_well_formed_instructions0 _ _ H2 _ _ H0 _ H1).
-      destruct i; auto. 
-      * simpl in H |-*.  destruct i; auto. 
+      destruct i; auto.
+      * simpl in H |-*.  destruct i; auto.
         destruct H as [bufs [Q1 Q2]].
-        exists bufs; intuition. 
+        exists bufs; intuition.
         rewrite PMapExtra.update_mapsto_iff. left; auto.
-      * simpl in H |-*. 
+      * simpl in H |-*.
         destruct H as [cprocs [pcode Q]].
         exists cprocs, pcode. intuition.
         rewrite PMapExtra.update_mapsto_iff. left; auto.
@@ -322,24 +331,24 @@ Proof.
         exists cprocs, P', PC; intuition.
         rewrite PMapExtra.update_mapsto_iff. left; auto.
       * simpl in H|-*.
-        destruct H. 
+        destruct H.
         intuition.
         unfold imported_procedure in *.
         destruct H3 as [CI Q].
         exists CI; intuition.
-        unfold Program.has_component in *. 
+        unfold Program.has_component in *.
         rewrite PMapExtra.update_mapsto_iff. left; auto.
-    - inv H2. destruct WF1. 
+    - inv H2. destruct WF1.
       pose proof (wfprog_well_formed_instructions0 _ _ H _ _ H0 _ H1).
-      destruct i; auto. 
-      * simpl in H2 |-*.  destruct i; auto. 
+      destruct i; auto.
+      * simpl in H2 |-*.  destruct i; auto.
         destruct H2 as [bufs [Q1 Q2]].
-        exists bufs; intuition. 
-        rewrite PMapExtra.update_mapsto_iff. right; intuition. 
+        exists bufs; intuition.
+        rewrite PMapExtra.update_mapsto_iff. right; intuition.
         eapply BDISJ; split; eauto.
         apply PMapFacts.find_mapsto_iff in Q1.
         apply PMapFacts.in_find_iff.  rewrite Q1; discriminate.
-      * simpl in H2 |-*. 
+      * simpl in H2 |-*.
         destruct H2 as [cprocs [pcode Q]].
         exists cprocs, pcode. intuition.
         rewrite PMapExtra.update_mapsto_iff. right; intuition.
@@ -348,15 +357,15 @@ Proof.
         exists cprocs, P', PC; intuition.
         rewrite PMapExtra.update_mapsto_iff. right; intuition.
       * simpl in H2 |-*.
-        destruct H2. 
+        destruct H2.
         split. auto.
         unfold imported_procedure in *.
         destruct H4 as [CI Q].
         exists CI; intuition.
-        unfold Program.has_component in *. 
-        rewrite PMapExtra.update_mapsto_iff. right; intuition. 
+        unfold Program.has_component in *.
+        rewrite PMapExtra.update_mapsto_iff. right; intuition.
         eapply IDISJ; split; eauto.
-        apply PMapFacts.find_mapsto_iff in H4. 
+        apply PMapFacts.find_mapsto_iff in H4.
         rewrite PMapFacts.in_find_iff. rewrite H4. discriminate.
   + Admitted. (* This obviously isn't true for arbitrary (mainC,mainP) ! *)
 *)
